reenable test and simplify another

Test/git-issues/git-issue-2500.dfy
@@ -50,32 +50,32 @@ module SSCinClass {
   trait Trait {
     predicate Even(i: nat)
     predicate Odd(i: nat)
-      ensures if i == 0 then true else (i % 2 == 1) == Even(i-1)
+      ensures i == 0 || (i % 2 == 1) == Even(i-1)
   }
 
   class Class extends Trait {
     predicate Even(i: nat)
-  { if i == 0 then true else Odd(i-1) }
+  { i == 0 || Odd(i-1) }
     predicate Odd(i: nat)
-      ensures if i == 0 then true else (i % 2 == 1) == Even(i-1)
-    { if i == 0 then false else Even(i-1) }
+      ensures i == 0 || (i % 2 == 1) == Even(i-1)
+    { i != 0 && Even(i-1) }
   }
 }
 
 module SSCinBoth {
   trait Trait {
     predicate Even(i: nat)
-      ensures if i == 0 then true else (i % 2 == 0) == Odd(i-1)
+      ensures i == 0 || (i % 2 == 0) == Odd(i-1)
     predicate Odd(i: nat)
-      ensures if i == 0 then true else (i % 2 == 1) == Even(i-1)
+      ensures i == 0 || (i % 2 == 1) == Even(i-1)
   }
 
   class Class extends Trait {
     predicate Even(i: nat)
-      ensures if i == 0 then true else (i % 2 == 0) == Odd(i-1)
-  { if i == 0 then true else Odd(i-1) }
+      ensures i == 0 || (i % 2 == 0) == Odd(i-1)
+  { i == 0 || Odd(i-1) }
     predicate Odd(i: nat)
-      ensures if i == 0 then true else (i % 2 == 1) == Even(i-1)
-    { if i == 0 then false else Even(i-1) }
+      ensures i == 0 || (i % 2 == 1) == Even(i-1)
+    { i != 0 && Even(i-1) }
   }
 }
