Test/dafny4/git-issue257.dfy
@@ -21,8 +21,7 @@ method Test0() {
 method Test1() {
   var c := new M.C();  // type is inferred to M.T? :(
   var g: M.T := c;
-  // Disabled until the type inference is fixed
-  // assert c.f() == 0;  // which used to cause this to fail, but shouldn't
+  assert c.f() == 0;  // which used to cause this to fail, but shouldn't
 }
 
 method Test2() {
